fairness/lawyer/obligations/obligations_wf.v
@@ -1,0 +1,610 @@
+Require Import Relation_Operators.
+From stdpp Require Import namespaces. 
+From trillium.fairness Require Import fairness locales_helpers utils.
+From trillium.fairness.lawyer.obligations Require Import obligations_model obls_utils multiset_utils.
+
+
+Section Wf.
+  Context `{OP: ObligationsParams Degree Level Locale LIM_STEPS}.
+  
+  Definition obls_assigned δ :=
+    dom $ filter (fun '(s, (l, b)) => b = false) (ps_sigs δ) ⊆
+    flatten_gset $ map_img $ ps_obls δ.
+
+  Definition dom_phases_disj δ :=
+    forall τ1 τ2 π1 π2, 
+      τ1 ≠ τ2 ->
+      ps_phases δ !! τ1 = Some π1 ->
+      ps_phases δ !! τ2 = Some π2 ->
+      phases_disj π1 π2. 
+
+  Definition eps_phase_bound δ :=
+    ¬ (exists τ π ep, ps_phases δ !! τ = Some π /\
+                  ep ∈ ps_eps δ /\ phase_lt π ep.1.2).
+
+  Definition cps_phase_bound δ :=
+    ¬ (exists τ π cp, ps_phases δ !! τ = Some π /\
+                  cp ∈ ps_cps δ /\ phase_lt π cp.1).
+
+  Definition obligations_are_signals δ :=
+    flatten_gset $ map_img $ ps_obls δ ⊆ dom $ ps_sigs δ. 
+
+  Definition obls_disjoint δ :=
+    forall τ1 τ2, τ1 ≠ τ2 -> 
+             default ∅ (ps_obls δ !! τ1) ## default ∅ (ps_obls δ !! τ2).   
+
+  Definition is_fork (π1 π2: Phase) := exists (d: nat), π2 = ext_phase π1 d. 
+
+  Lemma phase_le_ext_split π1 π2 d
+    (LE: phase_le π1 (ext_phase π2 d)):
+    π1 = ext_phase π2 d \/ phase_le π1 π2.
+  Proof using.
+    do 2 red in LE. destruct LE as [p EQ]. rewrite /ext_phase in EQ.
+    destruct p.
+    { simpl in EQ. eauto. }
+    rewrite -app_comm_cons in EQ. inversion EQ. subst.
+    right. red. red. exists p. eauto.
+  Qed. 
+
+  Record om_st_wf (δ: ProgressState) := {
+    om_wf_dpo: dom_phases_obls δ;
+    om_wf_asg: obls_assigned δ;
+    om_wf_ph_disj: dom_phases_disj δ;
+    om_wf_cps_ph_bound: cps_phase_bound δ;
+    om_wf_eps_ph_bound: eps_phase_bound δ;
+    om_wf_obls_are_sigs: obligations_are_signals δ;
+    om_wf_obls_disj: obls_disjoint δ;
+  }.
+
+  Definition preserved_by 
+    (R: ProgressState -> ProgressState -> Prop) (P: ProgressState -> Prop) :=
+    ∀ δ1 δ2, P δ1 -> R δ1 δ2 -> P δ2.
+  
+  Definition preserved_by_loc_step τ := preserved_by (loc_step_of τ).
+  Definition preserved_by_fork τ := preserved_by (fork_step_of τ).
+  Definition preserved_by_rep_loc_step τ :=
+    fun P => forall n, preserved_by (relations.nsteps (loc_step_of τ) n) P. 
+  Definition preserved_by_progress_step τ :=
+    preserved_by (progress_step_of τ). 
+  Definition preserved_by_om_trans τ :=
+    preserved_by (om_trans_of τ). 
+
+  Lemma pres_by_rel_implies_rep R P
+    (PRES: preserved_by R P)
+    :
+    forall n, preserved_by (relations.nsteps R n) P. 
+  Proof.
+    red. intros n. intros δ1.
+    induction n.
+    { simpl. intros ?? ->%nsteps_0. done. }
+    intros ?? (δ'&STEP1&STEP2)%rel_compose_nsteps_next.
+    apply IHn in STEP1; eauto.
+  Qed.
+
+  Lemma pres_by_loc_step_implies_rep τ P
+    (PRES: preserved_by_loc_step τ P)
+    :
+    preserved_by_rep_loc_step τ P. 
+  Proof.
+    red. intros. eapply pres_by_rel_implies_rep; eauto.
+  Qed.
+
+  Lemma pres_by_loc_step_implies_progress τ P
+    (PPRES: preserved_by_loc_step τ P)
+    :
+    preserved_by_progress_step τ P. 
+  Proof using.
+    do 2 red. intros δ1 δ2 P1 STEP. 
+    red in STEP. destruct STEP as (n&?&STEP).
+    eapply rel_compose_mono in STEP.
+    2: reflexivity.
+    1: apply rel_compose_nsteps_next in STEP.
+    2: { do 2 red. intros. by left. }    
+    eapply pres_by_loc_step_implies_rep; eauto.
+  Qed.
+
+  Lemma pres_by_loc_fork_steps_implies_om_trans τ P
+    (PPRES: preserved_by_loc_step τ P)
+    (FPRES: preserved_by_fork τ P)
+    :
+    preserved_by_om_trans τ P. 
+  Proof using.
+    do 2 red. intros δ1 δ2 P1 STEP. 
+    red in STEP. destruct STEP as (?&PSTEP&FSTEP).
+    eapply pres_by_loc_step_implies_progress in PPRES.
+    do 2 red in PPRES. specialize_full PPRES; eauto.
+    inversion FSTEP; subst; try done.
+    eapply FPRES; eauto. 
+  Qed.
+
+  Lemma pres_by_loc_fork_steps_implies_any_pres τ P
+    (PPRES: preserved_by_loc_step τ P)
+    (FPRES: preserved_by_fork τ P)
+    :
+    preserved_by (obls_any_step_of τ) P. 
+  Proof using.
+    red. intros ??? [? | ?]; eauto.
+  Qed. 
+
+  Lemma pres_by_valid_trace_strong (tr: obls_trace) i j P (T: Locale -> Prop)
+    (LE: i <= j)
+    (VALID: obls_trace_valid tr)
+    (PPRES: forall τ, T τ -> preserved_by_loc_step τ P)
+    (FPRES: forall τ, T τ -> preserved_by_fork τ P)
+    (Pi: from_option P True (tr S!! i))
+    (Tij: forall k τ, i <= k < j -> tr L!! k = Some τ -> T τ)
+    :
+    from_option P True (tr S!! j). 
+  Proof using.
+    apply Nat.le_sum in LE as [d ->]. induction d.
+    { rewrite Nat.add_0_r. done. }
+    rewrite -plus_n_Sm.
+    destruct (tr S!! S (i + d)) eqn:NEXT; [| done]. simpl.
+    forward eapply (proj1 (next_state_lookup _ _)); eauto.
+    intros [[? CUR] [? LBL]].
+    rewrite CUR in IHd. simpl in IHd.
+    forward eapply trace_valid_steps''; eauto.
+    { rewrite Nat.add_1_r. eauto. }
+    intros STEP.
+    pose proof (Tij (i + d) _ ltac:(lia) LBL).
+    eapply pres_by_loc_fork_steps_implies_om_trans; eauto.
+    2: { apply STEP. }
+    apply IHd. intros. eapply Tij; eauto. lia.  
+  Qed.
+
+  Lemma pres_by_valid_trace (tr: obls_trace) i P
+    (VALID: obls_trace_valid tr)
+    (PPRES: forall τ, preserved_by_loc_step τ P)
+    (FPRES: forall τ, preserved_by_fork τ P)
+    (Pi: from_option P True (tr S!! i)):
+    forall j, i <= j -> from_option P True (tr S!! j).
+  Proof using.
+    intros. eapply pres_by_valid_trace_strong with (T := fun _ => True); eauto.
+  Qed. 
+
+  Ltac inv_loc_step STEP :=
+    destruct STEP as [T|[T|[T|[T|[T|T]]]]];
+    [destruct T as (?&?&T) |
+     destruct T as (?&?&?&?&T) |
+     destruct T as (?&T) |
+     destruct T as (?&T) |
+     destruct T as (?&?&?&?&T) |
+     destruct T as (?&?&?&T) ];
+    inversion T; subst. 
+
+  Lemma loc_step_dpo_pres τ: preserved_by_loc_step τ dom_phases_obls.
+  Proof using.
+    do 2 red. intros δ1 δ2 PHASES_CORR STEP.
+    inv_loc_step STEP; destruct δ1; try done; simpl in *. 
+    - subst new_obls0. red. subst new_ps. simpl. set_solver. 
+    - subst new_obls0. simpl. red. set_solver. 
+  Qed.
+
+  Lemma loc_step_asg_pres τ: preserved_by_loc_step τ obls_assigned.
+  Proof using.
+    do 2 red. intros δ1 δ2 ASG STEP.
+    inv_loc_step STEP; destruct δ1; try done; simpl in *. 
+    - subst new_ps. red. simpl.
+      subst new_sigs0 new_obls0. 
+      rewrite map_filter_insert. setoid_rewrite decide_True; [| done].
+      rewrite dom_insert_L.
+      rewrite map_img_insert_L.
+      rewrite flatten_gset_union flatten_gset_singleton.
+      rewrite (union_comm_L _ {[ _ ]}) -union_assoc_L.
+      apply union_mono; [done| ]. etrans; [apply ASG| ].
+      simpl. rewrite {1}(map_img_sets_split_helper τ ps_obls). done. 
+    - subst new_ps. red. simpl.
+      subst new_sigs0 new_obls0.
+      rewrite map_filter_insert. setoid_rewrite decide_False; [| done].
+      rewrite map_img_insert_L.
+      rewrite flatten_gset_union flatten_gset_singleton.
+      apply elem_of_dom in DOM as [obls DOM].
+      subst cur_loc_obls0. rewrite DOM. simpl.
+
+      apply elem_of_subseteq. intros s' DOM'. rewrite elem_of_union. 
+      rewrite elem_of_dom in DOM'. destruct DOM' as [[l' b'] DOM'].
+      apply map_filter_lookup_Some in DOM' as [DOM' ->].
+      apply lookup_delete_Some in DOM' as [NEQ DOM'].
+      forward eapply (@ASG s').
+      { simpl. apply elem_of_dom. eexists.
+        eapply map_filter_lookup_Some; eauto. split; done. }
+      simpl. intros ASG'.
+      apply flatten_gset_spec in ASG'. destruct ASG' as (obls'&ASG'&IN').
+      apply elem_of_map_img in ASG' as [τ' ASG'].
+      destruct (decide (τ' = τ)) as [-> | ]. 
+      { rewrite DOM in ASG'. inversion ASG'. subst. set_solver. }
+      right. apply flatten_gset_spec. eexists. split; eauto.
+      apply elem_of_map_img. eexists. eapply lookup_delete_Some; eauto.
+  Qed.
+
+  Lemma loc_step_dpd_pres τ: preserved_by_loc_step τ dom_phases_disj.
+  Proof using.
+    do 2 red. intros δ1 δ2 DPD STEP.
+    inv_loc_step STEP; destruct δ1; try done; simpl in *.
+  Qed.
+
+  Definition phases_eq R δ1 := ps_phases δ1 = R.
+
+  Lemma loc_step_phases_pres τ R: preserved_by (loc_step_of τ) (phases_eq R).
+  Proof using. 
+    do 2 red. intros δ1 δ2 PH STEP.
+    inv_loc_step STEP; destruct δ1; try done; simpl in *.
+  Qed.
+
+  Lemma loc_step_epb_pres' τ: preserved_by_loc_step τ 
+                                (fun δ => eps_phase_bound δ /\ dom_phases_disj δ). 
+  Proof using.
+    do 2 red. intros δ1 δ2 [EPB DPD] STEP.
+    split.
+    2: { eapply loc_step_dpd_pres; eauto. } 
+    pose proof (@loc_step_phases_pres _ _ _ _ ltac:(reflexivity) STEP) as PH.
+    add_case (ps_eps δ2 ⊆ ps_eps δ1) EPS_LE.
+    { intros LE. red. intros (τ' & π & ep & PH2 & IN & LT).
+      eapply elem_of_subseteq in IN; eauto.
+      rewrite PH in PH2. 
+      edestruct EPB; eauto. set_solver. }
+    inv_loc_step STEP; destruct δ1; try done; simpl in *.
+    red. intros (τ' & π & ep & PH2 & IN & LT).
+    subst new_ps new_eps0. simpl in IN.
+    apply elem_of_union in IN as [IN | IN].
+    { edestruct EPB; eauto. set_solver. }
+    apply elem_of_singleton in IN as ->. (* simpl in *. *)
+    simpl in *.
+    assert (phase_lt π π__max) as LE'.
+    { eapply strict_transitive_l; eauto. } 
+    pose proof LE' as LE''%strict_include. 
+    eapply phases_disj_not_le in LE''; eauto.
+    eapply DPD; eauto.
+    intros ->. rewrite LOC_PHASE in PH2. inversion PH2. subst.
+    apply strict_spec_alt in LE'. tauto. 
+  Qed.
+
+  Lemma loc_step_cpb_pres' τ: preserved_by_loc_step τ
+                                (fun δ => cps_phase_bound δ /\ dom_phases_disj δ). 
+  Proof using.
+    do 2 red. intros δ1 δ2 [CPB DPD] STEP.
+    split.
+    2: by eapply loc_step_dpd_pres; eauto. 
+    pose proof (@loc_step_phases_pres _ _ _ _ ltac:(reflexivity) STEP) as PH.
+    add_case (ps_cps δ2 ⊆ ps_cps δ1) CPS_LE.
+    { intros LE. red. intros (τ' & π & cp & PH2 & IN & LT).
+      eapply gmultiset_elem_of_subseteq in IN; eauto.
+      rewrite PH in PH2. 
+      edestruct CPB; eauto. set_solver. }
+    
+    inv_loc_step STEP; destruct δ1; try done; simpl in *.
+    - apply CPS_LE. multiset_solver.
+    - red. simpl. intros (τ' & π & cp & PH2 & IN & LT).
+      subst new_cps0. rewrite gmultiset_elem_of_disj_union in IN.
+      destruct IN as [IN | IN].
+      { apply gmultiset_elem_of_weaken in IN.
+        edestruct CPB; eauto. set_solver. }
+      apply gmultiset_elem_of_scalar_mul in IN as [? IN].
+      apply gmultiset_elem_of_singleton in IN as ->. simpl in *.
+      edestruct CPB; eauto. set_solver.
+    - apply CPS_LE. multiset_solver.
+    - red. simpl. intros (τ' & π & cp & PH2 & IN & LT).
+      subst new_cps0. rewrite gmultiset_elem_of_disj_union in IN.
+      destruct IN as [IN | IN].
+      { edestruct CPB; eauto. set_solver. }
+      apply gmultiset_elem_of_singleton in IN as ->. simpl in *.
+      pose proof LT as LE''%strict_include. 
+      eapply phases_disj_not_le in LE''; eauto.
+      eapply DPD; eauto.
+      intros ->. rewrite LOC_PHASE in PH2. inversion PH2. subst.
+      apply strict_spec_alt in LT. tauto. 
+  Qed.
+
+  Lemma loc_step_obls_sigs_pres τ: preserved_by_loc_step τ obligations_are_signals.
+  Proof using.
+    do 2 red. intros δ1 δ2 OS STEP.
+    inv_loc_step STEP; destruct δ1; try done; simpl in *.
+    - subst new_ps. red. simpl. subst new_obls0 new_sigs0.
+      rewrite map_img_insert_L dom_insert_L.
+      rewrite flatten_gset_union flatten_gset_singleton.
+      rewrite (union_comm_L _ {[ _ ]}) -union_assoc_L.
+      apply union_mono; [done| ].
+      red in OS. simpl in OS.
+      etrans; [| apply OS].
+      rewrite {1}(map_img_sets_split_helper τ ps_obls). done.
+    - subst new_ps. red. simpl. subst new_obls0 new_sigs0.
+      etrans; [| etrans]; [| apply OS| ]; simpl.
+      2: { set_solver. }
+      rewrite map_img_insert_L.
+      rewrite flatten_gset_union flatten_gset_singleton.
+      rewrite {1}(map_img_sets_split_helper τ ps_obls). 
+      subst cur_loc_obls0. set_solver.
+  Qed. 
+
+  Lemma loc_step_obls_disj_pres' τ: preserved_by_loc_step τ
+                                      (fun δ => obls_disjoint δ /\ obligations_are_signals δ). 
+  Proof using.
+    do 2 red. intros δ1 δ2 [DPI OS] STEP.
+    split.
+    2: by eapply loc_step_obls_sigs_pres; eauto. 
+    inv_loc_step STEP; destruct δ1; try done; simpl in *.
+    - subst new_ps. red. simpl. intros τ1 τ2 NEQ.
+      subst new_obls0. simpl.
+
+      destruct (<[τ:=cur_loc_obls0 ∪ {[s0]}]> ps_obls !! τ1) eqn:L1, (<[τ:=cur_loc_obls0 ∪ {[s0]}]> ps_obls !! τ2) eqn:L2.
+      all: try set_solver. simpl.
+      rewrite !lookup_insert_Some in L1, L2. subst cur_loc_obls0.
+      destruct L1 as [(<- & EQ1) | (NEQ1 & EQ1)], L2 as [(<- & EQ2) | (NEQ2 & EQ2)]; try done. 
+      + subst g. apply disjoint_union_l. split.
+        * eapply disjoint_proper. 
+          3: eapply DPI; eauto.
+          ** simpl. done.
+          ** simpl. rewrite EQ2. done.
+        * apply disjoint_singleton_l. subst s0.
+          intros IN. destruct (next_sig_id_fresh (default ∅ (ps_obls !! τ) ∪ dom ps_sigs)).
+          apply elem_of_union_r. 
+          apply OS. simpl. apply flatten_gset_spec. eexists.
+          split; eauto. eapply elem_of_map_img; eauto.
+      + subst g0. apply disjoint_union_r. split.
+        * symmetry. eapply disjoint_proper. 
+          3: eapply DPI; eauto.
+          ** simpl. done.
+          ** simpl. rewrite EQ1. done.
+        * symmetry. apply disjoint_singleton_l. subst s0.
+          intros IN. edestruct (next_sig_id_fresh (default ∅ (ps_obls !! τ) ∪ dom ps_sigs)).
+          apply elem_of_union_r. apply OS. simpl.
+          apply flatten_gset_spec. eexists. split; eauto.
+          eapply elem_of_map_img; eauto. 
+      + forward eapply (DPI _ _ NEQ); eauto. simpl. rewrite EQ1 EQ2. set_solver.  
+    - subst new_ps. red. simpl. intros τ1 τ2 NEQ.
+      subst new_obls0. simpl.
+      eapply disjoint_subseteq; revgoals.
+      + eapply DPI; eauto.
+      + simpl. destruct (decide (τ2 = τ)) as [-> | ?].
+        * rewrite lookup_insert. set_solver.
+        * rewrite lookup_insert_ne; done.
+      + simpl. destruct (decide (τ1 = τ)) as [-> | ?].
+        * rewrite lookup_insert. set_solver.
+        * rewrite lookup_insert_ne; done.
+      + apply _. 
+  Qed.
+        
+  Lemma wf_preserved_by_loc_step τ: preserved_by (loc_step_of τ) om_st_wf.
+  Proof using.
+    red. intros ?? WF1 STEP. 
+    split.
+    - eapply loc_step_dpo_pres; eauto. apply WF1.
+    - eapply loc_step_asg_pres; eauto. apply WF1.  
+    - eapply loc_step_dpd_pres; eauto. apply WF1.
+    - eapply loc_step_cpb_pres'; eauto. split; apply WF1.
+    - eapply loc_step_epb_pres'; eauto. split; apply WF1.
+    - eapply loc_step_obls_sigs_pres; eauto. apply WF1.
+    - eapply loc_step_obls_disj_pres'; eauto. split; apply WF1.
+  Qed.
+
+  Lemma fork_step_obls_reorder δ1 τ δ2
+    (STEP: fork_step_of τ δ1 δ2)
+    (DPO1: dom_phases_obls δ1):
+    flatten_gset (map_img $ ps_obls δ2) = flatten_gset (map_img $ ps_obls δ1).
+  Proof using.
+    red in STEP. destruct STEP as (?&?&STEP).    
+    inversion STEP. subst.
+    assert (x ∉ dom $ ps_obls δ1) as FRESH''.
+    { rewrite -DPO1; auto. }
+    destruct δ1; subst; simpl in *.
+subst new_obls0.
+    rewrite map_img_insert_L. rewrite delete_insert_ne.
+    2: { intros ->. destruct FRESH'. by apply elem_of_dom. }
+    rewrite map_img_insert_L. 
+    rewrite (map_img_sets_split_helper x ps_obls).
+    rewrite not_elem_of_dom_1; [| done]. 
+    simpl. rewrite union_empty_l_L. erewrite !delete_notin with (i := x).
+    2: { by apply not_elem_of_dom. }
+    rewrite (map_img_sets_split_helper τ ps_obls).
+    rewrite !flatten_gset_union !flatten_gset_singleton.
+    rewrite union_assoc_L. f_equal. 
+    subst cur_obls0 obls' cur_obls.
+    destruct (ps_obls !! τ); simpl; [| set_solver].
+    apply set_eq. intros k. destruct (decide (k ∈ x0)); set_solver.
+  Qed.  
+
+  Lemma fork_step_dpo_pres τ:
+    preserved_by (fork_step_of τ) dom_phases_obls. 
+  Proof using.
+    do 2 red. intros δ1 δ2 ASG STEP. 
+    red in STEP. destruct STEP as (?&?&STEP).    
+    inversion STEP. subst.
+    destruct δ1; simpl in *.
+    subst new_phases0 new_obls0.
+    rewrite !dom_insert_L. set_solver.
+  Qed. 
+
+  Lemma fork_step_asg_pres' τ:
+    preserved_by (fun δ1 δ2 => fork_step_of τ δ1 δ2 /\ dom_phases_obls δ1) obls_assigned.
+  Proof using.
+    do 2 red. intros δ1 δ2 ASG [STEP WF1].
+    red in STEP. destruct STEP as (?&?&STEP).    
+    inversion STEP. subst.
+    erewrite fork_step_obls_reorder; eauto.
+    2: { red. eauto. }
+    destruct δ1; subst; simpl in *. done. 
+  Qed.
+
+  Lemma ext_phase_not_le π (i j: nat) (NEQ: i ≠ j):
+    ¬ phase_le (ext_phase π i) (ext_phase π j).
+  Proof using.
+    rewrite /ext_phase /phase_le.
+    intros. intros [p PREF].
+    destruct p; simpl in PREF. 
+    - inversion PREF. done.
+    - apply (f_equal length) in PREF. simpl in PREF.
+      rewrite app_length in PREF. simpl in PREF. lia.  
+  Qed. 
+
+  Lemma phases_disj_forks π (i j: nat) (NEQ: i ≠ j):
+    phases_disj (ext_phase π i) (ext_phase π j).
+  Proof using.
+    split; apply ext_phase_not_le; done. 
+  Qed.
+
+  Lemma phase_disj_ext π1 π2 (i: nat)
+    (DISJ: phases_disj π1 π2):
+    phases_disj (ext_phase π1 i) π2.
+  Proof using.
+    red. rewrite /ext_phase. split.  
+    - intros [p ->]. red in DISJ. apply proj1 in DISJ. edestruct DISJ; eauto.
+      rewrite cons_middle app_assoc. red. red. eauto.
+    - intros [p EQ]. red in DISJ.
+      destruct p.
+      { simpl in EQ. subst. apply proj1 in DISJ. edestruct DISJ; eauto.
+        red. red. exists [i]. eauto. }
+      rewrite -app_comm_cons in EQ. inversion EQ. subst.
+      apply proj2 in DISJ. edestruct DISJ; eauto.
+      red. red. exists p. eauto.
+  Qed. 
+
+  Lemma fork_step_dpd_pres τ:
+    preserved_by (fork_step_of τ) dom_phases_disj.
+  Proof using.
+    do 2 red. intros δ1 δ2 DPD STEP. 
+    red in STEP. destruct STEP as (?&?&STEP).    
+    inversion STEP. subst. subst ps'. simpl.
+    destruct δ1; simpl in *. subst new_phases0.
+    intros τ1 τ2 π1 π2. 
+    rewrite !lookup_insert_Some.    
+    intros NEQ [[-> <-] | [NEQ1 [[<- <-]| [NEQ1' PH1]]]] [[-> <-] | [NEQ2 [[<- <-]| [NEQ2' PH2]]]]; try tauto || by apply phases_disj_forks.
+    3, 4: symmetry.
+    1-3: by apply phase_disj_ext; eapply DPD; simpl; eauto. 
+    { apply phase_disj_ext. eapply DPD; [apply NEQ1'| ..]; eauto. }
+    eapply DPD; [apply NEQ|..]; eauto. 
+  Qed.
+
+  Lemma fork_step_cpb_pres τ: preserved_by (fork_step_of τ) cps_phase_bound.
+  Proof using.
+    do 2 red. intros δ1 δ2 CPB STEP. 
+    red in STEP. destruct STEP as (?&?&STEP).    
+    inversion STEP. subst. subst ps'. simpl.
+    destruct δ1; simpl in *. subst new_phases0.
+    repeat setoid_rewrite lookup_insert_Some.
+    intros (? & ? & ? & ([[-> <-] | [NEQ [[<- <-]| [NEQ' PH]]]] & IN & LT)).
+    - destruct CPB. exists τ. do 2 eexists. split; [| split]; eauto.
+      etrans; eauto. apply phase_lt_fork.
+    - destruct CPB. exists τ. do 2 eexists. split; [| split]; eauto.
+      etrans; eauto. apply phase_lt_fork.
+    - destruct CPB. exists x1. eauto.
+  Qed. 
+
+  Lemma fork_step_epb_pres τ: preserved_by (fork_step_of τ) eps_phase_bound.
+  Proof using.
+    do 2 red. intros δ1 δ2 EPB STEP. 
+    red in STEP. destruct STEP as (?&?&STEP).    
+    inversion STEP. subst. subst ps'. simpl.
+    destruct δ1; simpl in *. subst new_phases0.
+    repeat setoid_rewrite lookup_insert_Some.
+    intros (? & ? & ? & ([[-> <-] | [NEQ [[<- <-]| [NEQ' PH]]]] & IN & LT)).
+    - destruct EPB. exists τ. do 2 eexists. split; [| split]; eauto.
+      etrans; eauto. apply phase_lt_fork.
+    - destruct EPB. exists τ. do 2 eexists. split; [| split]; eauto.
+      etrans; eauto. apply phase_lt_fork.
+    - destruct EPB. exists x1. eauto.
+  Qed. 
+
+  Lemma fork_step_obls_sigs_pres τ: preserved_by (fun δ1 δ2 => fork_step_of τ δ1 δ2 /\ dom_phases_obls δ1) obligations_are_signals.
+  Proof using.
+    do 2 red. intros δ1 δ2 OS [STEP DPO1].
+    red in STEP. destruct STEP as (?&?&STEP).    
+    inversion STEP; subst.
+    erewrite fork_step_obls_reorder; eauto.
+    2: { red. eauto. }
+    destruct δ1; simpl in *. done.
+  Qed.
+
+  Lemma fork_step_obls_disj_pres τ:
+    preserved_by (fork_step_of τ) obls_disjoint. 
+  Proof using.
+    do 2 red. intros δ1 δ2 OS STEP. 
+    red in STEP. destruct STEP as (?&?&STEP).    
+    inversion STEP; subst.
+    destruct δ1; simpl in *. subst new_obls0.
+    intros τ1 τ2 NEQ. 
+    rewrite !insert_union_singleton_l !lookup_union.
+    rewrite !lookup_map_singleton.
+    
+    repeat destruct decide; subst; try tauto.
+    all: repeat rewrite union_Some_l; repeat rewrite option_union_left_id; simpl; subst obls' cur_obls cur_obls0.
+    - eapply disjoint_subseteq.
+      4: { apply OS, NEQ. }
+      { apply _. }
+      all: set_solver.
+    - set_solver. 
+    - eapply disjoint_subseteq.
+      4: { symmetry. apply OS, n1. }
+      { apply _. }
+      all: simpl; set_solver.
+    - set_solver.
+    - eapply disjoint_subseteq.
+      4: { symmetry. apply OS, n1. }
+      { apply _. }
+      all: simpl; set_solver.
+    - eapply disjoint_subseteq.
+      4: { apply OS, n0. }
+      { apply _. }
+      all: simpl; set_solver.
+    - eapply disjoint_subseteq.
+      4: { apply OS, n0. }
+      { apply _. }
+      all: simpl; set_solver.
+    - eapply disjoint_subseteq.
+      4: { apply OS, n0. }
+      { apply _. }
+      all: simpl; set_solver.
+    - eapply disjoint_subseteq; eauto. apply _. 
+  Qed.     
+
+  (* Lemma fork_step_cps_anc_pres τ: *)
+  (*   preserved_by (fork_step_of τ) cps_phases_ancestors. *)
+  (* Proof using. *)
+  (*   do 2 red. intros δ1 δ2 OS STEP.  *)
+  (*   red in STEP. destruct STEP as (?&?&STEP).     *)
+  (*   inversion STEP; subst. *)
+  (*   destruct δ1; simpl in *. subst new_obls0. *)
+  (*   subst new_phases0. rewrite map_img_insert_L. *)
+  (*   rewrite delete_notin. *)
+  (*   2: { apply not_elem_of_dom. rewrite dom_insert. *)
+  (*        apply not_elem_of_union. split; auto. *)
+  (*        apply not_elem_of_singleton. intros ->. *)
+  (*        destruct FRESH'. eapply elem_of_dom. eauto. } *)
+  (*   rewrite map_img_insert_L. *)
+  (*   intros ???.  *)
+  (*   rewrite !elem_of_union !elem_of_singleton. intros [->|[-> | OLD]] LE. *)
+  (*   -  *)
+
+    
+  Lemma wf_preserved_by_fork_step τ: preserved_by (fork_step_of τ) om_st_wf.
+  Proof using.
+    red. intros ?? WF1 STEP. 
+    split.
+    - eapply fork_step_dpo_pres; eauto. apply WF1.
+    - eapply fork_step_asg_pres'; [| split]; eauto; apply WF1.
+    - eapply fork_step_dpd_pres; eauto. apply WF1.
+    - eapply fork_step_cpb_pres; eauto. apply WF1.
+    - eapply fork_step_epb_pres; eauto. apply WF1.
+    - eapply fork_step_obls_sigs_pres; [| split]; eauto; apply WF1.
+    - eapply fork_step_obls_disj_pres; eauto. apply WF1.
+  Qed.
+
+  Lemma om_trans_wf_pres τ: preserved_by (om_trans_of τ) om_st_wf.
+  Proof using.
+    apply pres_by_loc_fork_steps_implies_om_trans.
+    - apply wf_preserved_by_loc_step.
+    - apply wf_preserved_by_fork_step.
+  Qed.
+    
+  Definition obls_eq R δ1 := dom $ ps_obls δ1 = R.
+      
+  Lemma loc_step_obls_pres R τ: preserved_by (loc_step_of τ) (obls_eq R). 
+  Proof using.
+    do 2 red. intros δ1 δ2 OE STEP. 
+    add_case (dom $ ps_obls δ2 = dom $ ps_obls δ1) SAME.
+    { intros EQ. by rewrite EQ. }
+    inv_loc_step STEP; destruct δ1; try done; simpl in *.
+    - subst new_obls0. rewrite dom_insert_L. simpl. set_solver.
+    - subst new_obls0. rewrite dom_insert_L. simpl. set_solver.
+  Qed.
+
+End Wf.
