fairness/lawyer/obligations/obls_refill_model.v
@@ -6,20 +6,19 @@ From trillium.fairness.lawyer.obligations Require Import obligations_model oblig
 
 
 Section RefillModel.
-  Context `(OP: ObligationsParams Degree Level Locale LIM_STEPS).
-  Context `{Countable Locale}.
+  Context `{OP: ObligationsParams Degree Level Locale LIM_STEPS}.
 
-  Let PS := ProgressState OP. 
+  Let PS := ProgressState.
 
   Inductive refills_cp: PS -> Locale -> PS -> Degree -> Prop :=
   | rcp_step ps τ δ π__max
-      (LOC_PHASE: ps_phases _ ps !! τ = Some π__max):
-    refills_cp ps τ (update_cps _ (ps_cps _ ps ⊎ {[+ (π__max, δ) +]}) ps) δ.
+      (LOC_PHASE: ps_phases ps !! τ = Some π__max):
+    refills_cp ps τ (update_cps (ps_cps ps ⊎ {[+ (π__max, δ) +]}) ps) δ.
 
   Definition om_refill_lbl := (Locale + Locale)%type. 
 
   Inductive obls_refill_trans: PS -> om_refill_lbl -> PS -> Prop :=
-  | ort_burn ps τ ps' (STEP: om_trans _ ps τ ps'):
+  | ort_burn ps τ ps' (STEP: om_trans ps τ ps'):
     obls_refill_trans ps (inl τ) ps'
   | ort_refill ps τ ps' δ (REFILL: refills_cp ps τ ps' δ):
     obls_refill_trans ps (inr τ) ps'
@@ -32,7 +31,7 @@ Section RefillModel.
   Definition refill_act: Action := coPpick (↑ refill_ns). 
 
   Inductive obls_refill_AM_trans: PS → Action * option om_refill_lbl → PS → Prop :=
-  | oram_burn δ1 ρ δ2 (STEP: om_trans _ δ1 ρ δ2):
+  | oram_burn δ1 ρ δ2 (STEP: om_trans δ1 ρ δ2):
     obls_refill_AM_trans δ1 (obls_act, Some (inl ρ)) δ2
   | oram_refill δ1 τ δ2 d (REFILL: refills_cp δ1 τ δ2 d):
     obls_refill_AM_trans δ1 (refill_act, Some (inr τ)) δ2
